DynamoDbItemEncryptor/src/DynamoToStruct.dfy
@@ -299,10 +299,10 @@ module DynamoToStruct {
       && (a.BOOL  ==> ret.Success? && |ret.value| == BOOL_LEN && ret.value[0] == 1)
       && (!a.BOOL ==> ret.Success? && |ret.value| == BOOL_LEN && ret.value[0] == 0)
     ensures a.BOOL? && prefix ==>
-      && (a.BOOL  ==> ret.Success? && |ret.value| == PREFIX_LEN+BOOL_LEN && ret.value[PREFIX_LEN] == 1
-          && ret.value[0..TYPEID_LEN] == BOOLEAN && ret.value[TYPEID_LEN..PREFIX_LEN] == [0,0,0,1])
-      && (!a.BOOL ==> ret.Success? && |ret.value| == PREFIX_LEN+BOOL_LEN && ret.value[PREFIX_LEN] == 0
-          && ret.value[0..TYPEID_LEN] == BOOLEAN && ret.value[TYPEID_LEN..PREFIX_LEN] == [0,0,0,1])
+      && (a.BOOL  ==> (ret.Success? && |ret.value| == PREFIX_LEN+BOOL_LEN && ret.value[PREFIX_LEN] == 1
+          && ret.value[0..TYPEID_LEN] == BOOLEAN && ret.value[TYPEID_LEN..PREFIX_LEN] == [0,0,0,1]))
+      && (!a.BOOL ==> (ret.Success? && |ret.value| == PREFIX_LEN+BOOL_LEN && ret.value[PREFIX_LEN] == 0
+          && ret.value[0..TYPEID_LEN] == BOOLEAN && ret.value[TYPEID_LEN..PREFIX_LEN] == [0,0,0,1]))
 
     //= specification/dynamodb-encryption-client/ddb-attribute-serialization.md#binary
     //= type=implication
